%!TEX root = ../main.tex
\documentclass[../main.tex]{subfiles}
\begin{document}
  \chapter{Proof of Steady State}\label{app:chap:derivation}
  \section{Change of Variables}\label{app:sec:cov}
  Starting with the McKendrick-von Foerster Equation with diffusion (\autoref{eq:mvf:diffusion}) we first need to change to a dimensionless variable $x = \log{w}$, so that $\varphi(x) \partial x = u(w) \partial w$. In a first step this gives that
  \begin{equation}
    \e{-x}\varphi_t = - (g(w) \e{-x} \varphi)_w - \e{-x} \mu(w) \varphi + \frac{1}{2}(D \e{-x}\varphi)_{ww}
  \end{equation}

  We then transform the derivatives from $w$ to $x$ using the chain rule
  \begin{equation}
    \frac{\partial}{\partial w}
    = \frac{\partial x}{\partial w} \frac{\partial}{\partial x} = \e{-x} \frac{\partial}{\partial x}.
  \end{equation}

  Which shows that
  \begin{eqnarray}
    \e{-x}\varphi_t
    &=& -\e{-x} \frac{\partial}{\partial x} \left(\hat{g} \varphi \right) - \e{-x} \hat{\mu}(x) \varphi + \frac{\e{-x}}{2} \frac{\partial}{\partial x} \left( \e{-x} \frac{\partial}{\partial x} \left( \hat{D} \varphi \right) \right) \nonumber \\
    \varphi_t
    &=& - \frac{\partial}{\partial x} \left(\hat{g} \varphi \right) - \hat{\mu}(x) \varphi + \frac{1}{2} \frac{\partial}{\partial x} \left( \e{-x} \frac{\partial}{\partial x} \left( \hat{D} \varphi \right) \right) \nonumber \\
    &=& - \left(\hat{g} \varphi \right)_x - \hat{\mu}(x) \varphi + \frac{\e{-x}}{2} \left( \left( \hat{D} \varphi \right)_{xx} - \left( \hat{D} \varphi \right)_x \right). \label{app:eq:cov}
  \end{eqnarray}

  Now we need to concentrate on the coefficient functions for growth, death and diffusion. First let us consider the growth function, $g(w)$ which from \autoref{sec:mvf:relation} takes the form
  \begin{equation}
    g(w) = \int K w' k(w, w') u(w') \: \mathrm{d} w' = \int K w' w^{\alpha} S \left( \frac{w}{w'} \right) u(w') \: \mathrm{d} w'
  \end{equation}

  then following the change of variables in \autoref{app:eq:cov} we take $\hat{g}(x) = \e{-x}g(\e{x})$, and since $\varphi(x) \partial x = u(w) \partial w$ we can change from $u$ to $\varphi$ in the integral very simply and thus
  \begin{equation}
    \hat{g}(x) = \e{-x} g(\e{x}) = \int K \e{x'} \e{(\alpha -1) x} \bar{S}( x - x' ) \varphi(x') \: \mathrm{d} x',
  \end{equation}

  where $\bar{S}(z) = S \left(\e{z} \right)$. Similarly for the diffusion coefficient
  \begin{equation}
    D(w) = \int (K w')^2 k(w, w') u(w') \: \mathrm{d} w' = \int (K w')^2 w^{\alpha} S \left( \frac{w}{w'} \right) u(w') \: \mathrm{d} w'
  \end{equation}

  we change variables so that
  \begin{equation}
    \hat{D}(x) = \e{-x} D(\e{x}) = \int K^2 \e{2x' + (\alpha-1) x} \bar{S}(x - x') \varphi(x') \: \mathrm{d} x'.
  \end{equation}

  The death term provides an easier change of variables with
  \begin{equation}
    \hat{\mu}(x) = \mu(\e{x}) = \int \e{\alpha x'} \bar{S}(x' - x) \varphi(x') \: \mathrm{d}x' - \delta.
  \end{equation}

  If we now assume that $\e{\gamma x} \rho(x) = \varphi(x)$, so that if the steady state of $\varphi(x) \propto \e{\gamma x}$ then the steady state of $\rho(x) \propto 1$, then we have that \autoref{app:eq:cov} implies

  \begin{eqnarray}
    \e{\gamma x} \rho_t
    &=& - (\hat{g} \e{\gamma x} \rho)_x - \hat{\mu} \e{\gamma x} \rho + \frac{\e{-x}}{2} \left( (\hat{D}\e{\gamma x} \rho)_{xx} - (\hat{D} \e{\gamma x} \rho)_x \right) \nonumber \\
    &=& - (\bar{g} \rho)_x - \bar{\mu} \e{\gamma x} \rho + \frac{\e{-x}}{2} \left( (\bar{D} \rho)_{xx} - (\bar{D} \rho)_x \right)
  \end{eqnarray}

  with the coefficient equations
  \begin{eqnarray}
    \bar{g}(x) &=& \int K \e{(\gamma + 1) x' + (\gamma + \alpha - 1) x} \bar{S}( x - x' ) \rho(x') \: \mathrm{d} x' \\
    \bar{D}(x) &=& \int K^2 \e{(\gamma + 2) x' + (\gamma + \alpha - 1) x} \bar{S}( x - x' ) \rho(x') \: \mathrm{d} x' \\
    \bar{\mu}(x) &=& \int \e{(\alpha + \gamma) x'} \bar{S}(x' - x)\rho(x') \: \mathrm{d}x' - \delta
  \end{eqnarray}

  If we then follow the example of \cite{datta2011} and set $\alpha + \gamma - 1 = 0$, then these are reduced to
  \begin{eqnarray}
    \bar{g}(x)
    &=& \int K \e{(\gamma + 1) x'} \bar{S}( x - x' ) \rho(x') \: \mathrm{d} x' \nonumber \\
    &=& \int K \e{(\gamma + 1)(x-y)} \bar{S}(y) \rho(x-y) \: \mathrm{d}y \\
    \bar{D}(x)
    &=& \int K^2 \e{(\gamma + 2) x'} \bar{S}( x - x' ) \rho(x') \: \mathrm{d} x' \nonumber \\
    &=& \int K^2 \e{(\gamma + 2)(x-y)} \bar{S}(y) \rho(x-y) \: \mathrm{d}y \\
    \bar{\mu}(x)
    &=& \int \e{x'} \bar{S}(x' - x)\rho(x') \: \mathrm{d}x' - \delta \nonumber \\
    &=& - \int \e{x+y} \bar{S}(y) \rho(x+y) \: \mathrm{d}y - \delta
  \end{eqnarray}

  \section{Steady State Condition}
  At steady state we have that $\varphi(x) = \varphi_0 \e{\gamma x}$, so $\rho(x) = \upsilon_0 = \varphi_0$, thus we have that, after cancelling $\upsilon_0$
  \begin{equation}
    0 =  \e{-\gamma x}\bar{g}_x + \bar{\mu} - \frac{\e{-(\gamma + 1) x}}{2} \left( \bar{D}_{xx} - \bar{D}_x \right)
  \end{equation}

  which, after substituting in the coefficient functions and cancelling some overall factors gives a steady state condition for the equation.
  \begin{equation}
    \int \bar{S}(y) \e{x+y} \left( -1 + (\gamma +1)K\e{-(\gamma + 2)y} - (\gamma +2 )(\gamma +3) \frac{K^2}{2}\e{-(\gamma + 3)y} \right) \: \mathrm{d}y - \eta
  \end{equation}

\end{document}
